coq/config.el
@@ -1,2 +1,1 @@
-(setq coq-prog-args (list "-dont-load-proofs"))
-(setq coq-load-path (list (list (expand-file-name default-directory) "LCAC")))
+(add-to-list 'coq-load-path (list (expand-file-name default-directory) "LCAC"))
